<?xml version="1.0" encoding="utf-8" ?>
<rdf:RDF xmlns:rdf="http://www.w3.org/1999/02/22-rdf-syntax-ns#"
         xmlns:rdfs="http://www.w3.org/2000/01/rdf-schema#"
         xmlns:dc="http://purl.org/dc/terms/"
         xmlns:owl="http://www.w3.org/2002/07/owl#">

  <rdfs:Description rdf:about="http://cola.jackflaps.net/cola#">
    <dc:title>Colorado Local Authorities data dictionary</dc:title>
    <dc:publisher>University of Denver</dc:publisher>
    <owl:versionInfo>0.1</owl:versionInfo>
    <rdfs:comment>Data dictionary for the Colorado Local Authorities linked archival data project</rdfs:comment>
  </rdfs:Description>

  <rdfs:Class rdf:about="http://cola.jackflaps.net/cola#agent">
    <rdfs:isDefinedBy>http://cola.jackflaps.net/cola#</rdfs:isDefinedBy>
    <rdfs:label>Agent</rdfs:label>
    <rdfs:comment>The general CoLA agent class</rdfs:comment>
  </rdfs:Class>

  <rdfs:Class rdf:about="http://cola.jackflaps.net/cola#identity">
    <rdfs:isDefinedBy>http://cola.jackflaps.net/cola#</rdfs:isDefinedBy>
    <rdfs:label>Identity</rdfs:label>
    <rdfs:comment>The class of identities by which a cola:agent is known. ISAAR(CPF) 5.1</rdfs:comment>
  </rdfs:Class>

  <rdfs:Class rdf:about="http://cola.jackflaps.net/cola#relation">
    <rdfs:isDefinedBy>http://cola.jackflaps.net/cola#</rdfs:isDefinedBy>
    <rdfs:label>Relationship</rdfs:label>
    <rdfs:comment>The class of relationships between cola:agents and the resources of which they are creator or subject. ISAAR(CPF) 5.3</rdfs:comment>
  </rdfs:Class>

  <rdfs:Class rdf:about="http://cola.jackflaps.net/cola#place">
    <rdfs:isDefinedBy>http://cola.jackflaps.net/cola#</rdfs:isDefinedBy>
    <rdfs:label>Place</rdfs:label>
    <rdfs:comment>The class of geographic locations of relevance to the cola:agent being described. ISAAR(CPF) 5.2.3</rdfs:comment>
  </rdfs:Class>

  <rdfs:Class rdf:about="http://cola.jackflaps.net/cola#date">
    <rdfs:isDefinedBy>http://cola.jackflaps.net/cola#</rdfs:isDefinedBy>
    <rdfs:label>Date</rdfs:label>
    <rdfs:comment>The class of dates of relevance to the cola:agent being described.</rdfs:comment>
  </rdfs:Class>

  <rdfs:Class rdf:about="http://cola.jackflaps.net/cola#maintenanceEvent">
    <rdfs:isDefinedBy>http://cola.jackflaps.net/cola#</rdfs:isDefinedBy>
    <rdfs:label>Maintenance Event</rdfs:label>
    <rdfs:comment>The class of events associated with the creation and ongoing maintenance of a cola:agent representation. ISAAR(CPF) 5.4.6, 5.4.9</rdfs:comment>
  </rdfs:Class>

  <rdf:Property rdf:about="http://cola.jackflaps.net/cola#hasIdentity">
    <rdfs:domain rdf:resource="http://cola.jackflaps.net/cola#agent"/>
    <rdfs:range rdf:resource="http://cola.jackflaps.net/cola#identity"/>
    <rdfs:label>has identity</rdfs:label>
    <rdfs:comment>The property indicating the existence of a relationship between an agent and an identity for that agent.</rdfs:comment>
  </rdf:Property>

  <rdf:Property rdf:about="http://cola.jackflaps.net/cola#hasPlace">
    <rdfs:domain rdf:resource="http://cola.jackflaps.net/cola#agent"/>
    <rdfs:range rdf:resource="http://cola.jackflaps.net/cola#place"/>
    <rdfs:label>has place</rdfs:label>
    <rdfs:comment>The property indicating the existence of a relationship between an agent and a geographical location.</rdfs:comment>
  </rdf:Property>

  <rdf:Property rdf:about="http://cola.jackflaps.net/cola#hasDate">
    <rdfs:domain rdf:resource="http://cola.jackflaps.net/cola#agent"/>
    <rdfs:range rdf:resource="http://cola.jackflaps.net/cola#date"/>
    <rdfs:label>has date</rdfs:label>
    <rdfs:comment>The property indicating a date of importance in the biography or history of an agent.</rdfs:comment>
  </rdf:Property>

  <rdf:Property rdf:about="http://cola.jackflaps.net/cola#hasRelation">
    <rdfs:domain rdf:resource="http://cola.jackflaps.net/cola#agent"/>
    <rdfs:range rdf:resource="http://cola.jackflaps.net/cola#relation"/>
    <rdfs:label>has relationship</rdfs:label>
    <rdfs:comment>The property indicating a relationship between two agents.</rdfs:comment>
  </rdf:Property>

  <rdf:Property rdf:about="http://cola.jackflaps.net/cola#hasMaintenanceEvent">
    <rdfs:domain rdf:resource="http://cola.jackflaps.net/cola#agent"/>
    <rdfs:range rdf:resource="http://cola.jackflaps.net/cola#maintenanceEvent"/>
    <rdfs:label>has maintenance event</rdfs:label>
    <rdfs:comment>The property indicating the existence of a maintenance event for a cola:agent representation.</rdfs:comment>
  </rdf:Property>

  <rdf:Property rdf:about="http://cola.jackflaps.net/cola#hasType">
    <rdfs:domain rdf:resource="http://cola.jackflaps.net/cola#agent"/>
    <rdfs:label>has type</rdfs:label>
    <rdfs:comment>The type of agent represented: person, corporate body, family, software.</rdfs:comment>
  </rdf:Property>

  <rdf:Property rdf:about="http://cola.jackflaps.net/cola#hasOccupation">
    <rdfs:domain rdf:resource="http://cola.jackflaps.net/cola#agent"/>
    <rdfs:label>has occupation</rdfs:label>
    <rdfs:comment>An occupation held by an agent.</rdfs:comment>
  </rdf:Property>

  <rdf:Property rdf:about="http://cola.jackflaps.net/cola#hasFunction">
    <rdfs:domain rdf:resource="http://cola.jackflaps.net/cola#agent"/>
    <rdfs:label>has function</rdfs:label>
    <rdfs:comment>The funciton performed by an agent</rdfs:comment>
  </rdf:Property>

  <rdf:Property rdf:about="http://cola.jackflaps.net/cola#hasBiogHist">
    <rdfs:domain rdf:resource="http://cola.jackflaps.net/cola#agent"/>
    <rdfs:label>biography</rdfs:label>
    <rdfs:comment>The biography or history of the described agent</rdfs:comment>
  </rdf:Property>

  <rdf:Property rdf:about="http://cola.jackflaps.net/cola#hasPart">
    <rdfs:domain rdf:resource="http://cola.jackflaps.net/cola#identity"/>
    <rdfs:label>has part</rdfs:label>
    <rdfs:comment>A semantically ambiguous part of name of the described identity</rdfs:comment>
  </rdf:Property>

  <rdf:Property rdf:about="http://cola.jackflaps.net/cola#hasSurname">
    <rdfs:domain rdf:resource="http://cola.jackflaps.net/cola#identity"/>
    <rdfs:label>has surname</rdfs:label>
    <rdfs:comment>The surname of the described identity</rdfs:comment>
  </rdf:Property>

  <rdf:Property rdf:about="http://cola.jackflaps.net/cola#hasForename">
    <rdfs:domain rdf:resource="http://cola.jackflaps.net/cola#identity"/>
    <rdfs:label>has forename</rdfs:label>
    <rdfs:comment>The forename of the described identity</rdfs:comment>
  </rdf:Property>

  <rdf:Property rdf:about="http://cola.jackflaps.net/cola#hasPrefix">
    <rdfs:domain rdf:resource="http://cola.jackflaps.net/cola#identity"/>
    <rdfs:label>has prefix</rdfs:label>
    <rdfs:comment>The prefix of the described identity</rdfs:comment>
  </rdf:Property>

  <rdf:Property rdf:about="http://cola.jackflaps.net/cola#hasSuffix">
    <rdfs:domain rdf:resource="http://cola.jackflaps.net/cola#identity"/>
    <rdfs:label>has suffix</rdfs:label>
    <rdfs:comment>The suffix of the described identity</rdfs:comment>
  </rdf:Property>

  <rdf:Property rdf:about="http://cola.jackflaps.net/cola#hasPrimary">
    <rdfs:domain rdf:resource="http://cola.jackflaps.net/cola#identity"/>
    <rdfs:label>has primary</rdfs:label>
    <rdfs:comment>The primary form of name of the described identity</rdfs:comment>
  </rdf:Property>

  <rdf:Property rdf:about="http://cola.jackflaps.net/cola#hasSubordinate">
    <rdfs:domain rdf:resource="http://cola.jackflaps.net/cola#identity"/>
    <rdfs:label>has subordinate</rdfs:label>
    <rdfs:comment>The subordinate form(s) of name of the described identity</rdfs:comment>
  </rdf:Property>

  <rdf:Property rdf:about="http://cola.jackflaps.net/cola#hasForm">
    <rdfs:domain rdf:resource="http://cola.jackflaps.net/cola#identity"/>
    <rdfs:label>has form</rdfs:label>
    <rdfs:comment>The form of name described within the cola:identity: authorized, alternative, parallel, variant.</rdfs:comment>
  </rdf:Property>

  <rdf:Property rdf:about="http://cola.jackflaps.net/cola#hasRules">
    <rdfs:domain rdf:resource="http://cola.jackflaps.net/cola#identity"/>
    <rdfs:label>has rules</rdfs:label>
    <rdfs:comment>The cataloging rules, if any, by which the identity was constructed: DACS, AACR2, RDA, etc.</rdfs:comment>
  </rdf:Property>

  <rdf:Property rdf:about="http://cola.jackflaps.net/cola#hasUseDates">
    <rdfs:domain rdf:resource="http://cola.jackflaps.net/cola#identity"/>
    <rdfs:range rdf:resource="http://cola.jackflaps.net/cola#date"/>
    <rdfs:label>has use dates</rdfs:label>
    <rdfs:comment>The dates during which the identity form described was used to name the represented agent</rdfs:comment>
  </rdf:Property>

  <rdf:Property rdf:about="http://cola.jackflaps.net/cola#relationType">
    <rdfs:domain rdf:resource="http://cola.jackflaps.net/cola#relation"/>
    <rdfs:label>relation type</rdfs:label>
    <rdfs:comment>The high-level relationship described by the cola:relation, according to EAC-CPF terminology</rdfs:comment>
  </rdf:Property>

  <rdf:Property rdf:about="http://cola.jackflaps.net/cola#relationEntry">
    <rdfs:domain rdf:resource="http://cola.jackflaps.net/cola#relation"/>
    <rdfs:label>relation entry</rdfs:label>
    <rdfs:comment>The related agent</rdfs:comment>
  </rdf:Property>

  <rdf:Property rdf:about="http://cola.jackflaps.net/cola#relationship">
    <rdfs:domain rdf:resource="http://cola.jackflaps.net/cola#relation"/>
    <rdfs:label>relationship</rdfs:label>
    <rdfs:comment>The specific type of relationship described by the cola:relation, narrower in scope than its cola:relationType</rdfs:comment>
  </rdf:Property>

  <rdf:Property rdf:about="http://cola.jackflaps.net/cola#placeEntry">
    <rdfs:domain rdf:resource="http://cola.jackflaps.net/cola#place"/>
    <rdfs:label>place entry</rdfs:label>
    <rdfs:comment>The place associated with the agent's cola:hasPlace relationship</rdfs:comment>
  </rdf:Property>

  <rdf:Property rdf:about="http://cola.jackflaps.net/cola#placeRole">
    <rdfs:domain rdf:resource="http://cola.jackflaps.net/cola#place"/>
    <rdfs:label>place role</rdfs:label>
    <rdfs:comment>The role played by the place in the existence of the agent</rdfs:comment>
  </rdf:Property>

  <rdf:Property rdf:about="http://cola.jackflaps.net/cola#singleDate">
    <rdfs:domain rdf:resource="http://cola.jackflaps.net/cola#date"/>
    <rdfs:label>single date</rdfs:label>
    <rdfs:comment>A single date associated with the agent</rdfs:comment>
  </rdf:Property>

  <rdf:Property rdf:about="http://cola.jackflaps.net/cola#fromDate">
    <rdfs:domain rdf:resource="http://cola.jackflaps.net/cola#date"/>
    <rdfs:label>date from</rdfs:label>
    <rdfs:comment>The first date in a date range associated with the agent</rdfs:comment>
  </rdf:Property>

  <rdf:Property rdf:about="http://cola.jackflaps.net/cola#toDate">
    <rdfs:domain rdf:resource="http://cola.jackflaps.net/cola#date"/>
    <rdfs:label>date to</rdfs:label>
    <rdfs:comment>The last date in a date range associated with the agent</rdfs:comment>
  </rdf:Property>

  <rdf:Property rdf:about="http://cola.jackflaps.net/cola#dateNote">
    <rdfs:domain rdf:resource="http://cola.jackflaps.net/cola#date"/>
    <rdfs:label>date note</rdfs:label>
    <rdfs:comment>A note providing additional details about the date or date range as it pertains to the agent described</rdfs:comment>
  </rdf:Property>

  <rdf:Property rdf:about="http://cola.jackflaps.net/cola#eventType">
    <rdfs:domain rdf:resource="http://cola.jackflaps.net/cola#maintenanceEvent"/>
    <rdfs:label>event type</rdfs:label>
    <rdfs:comment>The type of maintenance event associated with the CoLA record</rdfs:comment>
  </rdf:Property>

  <rdf:Property rdf:about="http://cola.jackflaps.net/cola#eventDate">
    <rdfs:domain rdf:resource="http://cola.jackflaps.net/cola#maintenanceEvent"/>
    <rdfs:label>event date</rdfs:label>
    <rdfs:comment>The date and time at which the event was performed or generated</rdfs:comment>
  </rdf:Property>

  <rdf:Property rdf:about="http://cola.jackflaps.net/cola#eventDescription">
    <rdfs:domain rdf:resource="http://cola.jackflaps.net/cola#maintenanceEvent"/>
    <rdfs:label>event description</rdfs:label>
    <rdfs:comment>A detailed description of the event</rdfs:comment>
  </rdf:Property>

  <rdf:Property rdf:about="http://cola.jackflaps.net/cola#eventAgentType">
    <rdfs:domain rdf:resource="http://cola.jackflaps.net/cola#maintenanceEvent"/>
    <rdfs:label>event agent type</rdfs:label>
    <rdfs:comment>Whether the agent performing the event was a human or a machine</rdfs:comment>
  </rdf:Property>

  <rdf:Property rdf:about="http://cola.jackflaps.net/cola#eventAgent">
    <rdfs:domain rdf:resource="http://cola.jackflaps.net/cola#maintenanceEvent"/>
    <rdfs:label>event agent</rdfs:label>
    <rdfs:comment>The agent responsible for performing the maintenance event</rdfs:comment>
  </rdf:Property>

</rdf:RDF>
